Logic/Modal/Standard/Kripke/ModalCompanion.lean
@@ -107,7 +107,7 @@ lemma provable_S4_of_provable_efq : (𝐒𝟒 ⊢! pᵍ) → (𝐈𝐧𝐭 ⊢! 
   intro h;
   obtain ⟨iF, _, iV, iV_hereditary, w, h⟩ := by simpa [ValidOnFrameClass, ValidOnFrame, ValidOnModel] using not_imp_not.mpr Superintuitionistic.Kripke.complete! h;
 
-  let M : Modal.Standard.Kripke.Model iF.World α := { Frame := { Rel := iF.Rel }, Valuation := iV };
+  let M : Modal.Standard.Kripke.Model α := { Frame := { Rel := iF.Rel }, Valuation := iV };
   have h₁ : ∀ q v, Satisfies ⟨iF, iV, iV_hereditary⟩ v q ↔ (Modal.Standard.Formula.kripke_satisfies M v (qᵍ)) := by
     intro q v;
     induction q using Superintuitionistic.Formula.rec' generalizing v with
@@ -123,7 +123,7 @@ lemma provable_S4_of_provable_efq : (𝐒𝟒 ⊢! pᵍ) → (𝐈𝐧𝐭 ⊢! 
 
   apply not_imp_not.mpr $ Modal.Standard.Kripke.sound_S4.sound;
   simp [Formula.valid_on_KripkeFrame, valid_on_KripkeModel];
-  use M.World, M.Frame;
+  use M.Frame;
   exact ⟨
     iF.Rel_refl,
     iF.Rel_trans,
