Logic/Modal/Standard/Kripke/Preservation.lean
@@ -9,7 +9,7 @@ namespace Kripke
 
 section Bisimulation
 
-structure Model.Bisimulation (M₁ : Kripke.Model δ₁ α) (M₂ : Kripke.Model δ₂ α) where
+structure Model.Bisimulation (M₁ M₂ : Kripke.Model α) where
   toRel : Rel M₁.World M₂.World
   atomic {x₁ : M₁.World} {x₂ : M₂.World} {a : α} : toRel x₁ x₂ → ((M₁.Valuation x₁ a) ↔ (M₂.Valuation x₂ a))
   forth {x₁ y₁ : M₁.World} {x₂ : M₂.World} : toRel x₁ x₂ → x₁ ≺ y₁ → ∃ y₂ : M₂.World, toRel y₁ y₂ ∧ x₂ ≺ y₂
@@ -25,12 +25,12 @@ end Bisimulation
 section ModalEquivalent
 
 
-def ModalEquivalent (M₁ : Kripke.Model δ₁ α) (M₂ : Kripke.Model δ₂ α) (w₁ : M₁.World) (w₂ : M₂.World) : Prop := ∀ p, w₁ ⊧ p ↔ w₂ ⊧ p
+def ModalEquivalent (M₁ M₂ : Kripke.Model α) (w₁ : M₁.World) (w₂ : M₂.World) : Prop := ∀ p, w₁ ⊧ p ↔ w₂ ⊧ p
 notation:max "("  M₁ "," w₁ ")" " ↭ " "("  M₂ "," w₂ ")" => ModalEquivalent M₁ M₂ w₁ w₂
 
 open Formula
 
-variable {M₁ : Kripke.Model δ₁ α} {M₂ : Kripke.Model δ₂ α}
+variable {M₁ M₂ : Kripke.Model α}
 variable (Bi : M₁ ⇄ M₂)
 
 lemma modal_equivalent_of_bisimilar (bisx : Bi x₁ x₂) : (M₁, x₁) ↭ (M₂, x₂) := by
@@ -87,7 +87,7 @@ section PseudoEpimorphism
 variable {δ₁ δ₂}
 
 /-- As known as _p-morphism_. -/
-structure Frame.PseudoEpimorphism (F₁ : Kripke.Frame δ₁) (F₂ : Kripke.Frame δ₂) where
+structure Frame.PseudoEpimorphism (F₁ F₂ : Kripke.Frame) where
   toFun : F₁.World → F₂.World
   forth {x y : F₁.World} : x ≺ y → toFun x ≺ toFun y
   back {w : F₁.World} {v : F₂.World} : toFun w ≺ v → ∃ u, toFun u = v ∧ w ≺ u
@@ -97,7 +97,7 @@ infix:80 " →ₚ " => Frame.PseudoEpimorphism
 instance : CoeFun (Frame.PseudoEpimorphism F₁ F₂) (λ _ => F₁.World → F₂.World) := ⟨λ f => f.toFun⟩
 
 
-structure Model.PseudoEpimorphism (M₁ : Kripke.Model δ₁ α) (M₂ : Kripke.Model δ₂ α) extends M₁.Frame →ₚ M₂.Frame where
+structure Model.PseudoEpimorphism (M₁ M₂ : Kripke.Model α) extends M₁.Frame →ₚ M₂.Frame where
   atomic {w : M₁.World} {a} : (M₁.Valuation w a) ↔ (M₂.Valuation (toFun w) a)
 
 infix:80 " →ₚ " => Model.PseudoEpimorphism
@@ -107,8 +107,8 @@ instance : CoeFun (Model.PseudoEpimorphism M₁ M₂) (λ _ => M₁.World → M�
 
 open Formula
 
-variable {F₁ : Kripke.Frame δ₁} {F₂ : Kripke.Frame δ₂}
-         {M₁ : Kripke.Model δ₁ α} {M₂ : Kripke.Model δ₂ α}
+variable {F₁ F₂ : Kripke.Frame}
+         {M₁ M₂ : Kripke.Model α}
          {p : Formula α}
 
 lemma iff_formula_satisfies_morphism (f : M₁ →ₚ M₂) {w : M₁.World}
@@ -137,8 +137,8 @@ lemma iff_formula_valid_on_frame_surjective_morphism (f : F₁ →ₚ F₂) (f_s
   let V₁ := λ w a => V₂ (f w) a;
   use V₁, w₁;
 
-  let M₁ : Model δ₁ α := { Frame := F₁, Valuation := V₁ };
-  let M₂ : Model δ₂ α := { Frame := F₂, Valuation := V₂ };
+  let M₁ : Model α := { Frame := F₁, Valuation := V₁ };
+  let M₂ : Model α := { Frame := F₂, Valuation := V₂ };
   exact iff_formula_satisfies_morphism (M₁ := M₁) (M₂ := M₂) {
     toFun := f,
     forth := f.forth,
@@ -151,16 +151,16 @@ lemma iff_theory_valid_on_frame_surjective_morphism (f : F₁ →ₚ F₂) (f_su
   intro h p hp;
   exact iff_formula_valid_on_frame_surjective_morphism f f_surjective (h hp);
 
-abbrev IrreflexiveFrameClass : FrameClass := λ ⟨_, F⟩ => Irreflexive F
+abbrev IrreflexiveFrameClass : FrameClass := { F | Irreflexive F }
 
 theorem undefinable_irreflexive : ¬∃ (Ax : AxiomSet α), AxiomSet.DefinesKripkeFrameClass.{_, 0} Ax IrreflexiveFrameClass := by
   by_contra hC;
   obtain ⟨Ax, h⟩ := hC;
 
-  let F₁ : Frame (Fin 2) := { Rel := (· ≠ ·) };
+  let F₁ : Frame := { World := Fin 2, Rel := (· ≠ ·) };
   have hIF₁ : Irreflexive F₁ := by simp [Irreflexive, Frame.Rel'];
 
-  let F₂ : Frame (Fin 1) := { Rel := (· = ·) };
+  let F₂ : Frame := { World := Fin 1, Rel := (· = ·) };
 
   let f : F₁ →ₚ F₂ := {
     toFun := λ _ => 0,
@@ -169,8 +169,8 @@ theorem undefinable_irreflexive : ¬∃ (Ax : AxiomSet α), AxiomSet.DefinesKrip
       simp;
       intro w;
       match w with
-      | 0 => use 1; simp [Frame.Rel'];
-      | 1 => use 0; simp [Frame.Rel'];
+      | 0 => use 1;
+      | 1 => use 0;
   };
   have f_surjective : Function.Surjective f := by simp [Function.Surjective]; aesop;
 
